Make [Tenum] a constructor.
The C++ standard states the [enum] generates a new type.
- We deviate slightly from the C++ AST by ensuring that a reference
  to an enum constant always has the type of the enum constant, regardless
  of where it occurs.
- We insert [Cintegral] casts to make expressions work out.

theories/lang/cpp/parser.v
@@ -51,8 +51,6 @@ Definition Sforeach (range ibegin iend : Stmt)
 (* Indicate that [underlying] is used to represent alias type [name]. Enums are treated similarly. *)
 Definition Talias (name : globname) {underlying : type} : type :=
   underlying.
-Definition Tenum (name : globname) {underlying : type} : type :=
-  underlying.
 Definition Tunderlying (enum : type) {underlying : type} : type :=
   underlying.
 
