theories/lang/cpp/logic/expr.v
@@ -272,9 +272,12 @@ Module Type Expr.
     Axiom wp_operand_unop : forall o e ty Q,
         wp_operand e (fun v free => (* todo: rval? *)
           Exists v',
-          [| eval_unop o (drop_qualifiers (type_of e)) (drop_qualifiers ty) v v' |] **
+          [| exists tu, tu ⊧ resolve /\ eval_unop tu o (drop_qualifiers (type_of e)) (drop_qualifiers ty) v v' |] **
           Q v' free)
         |-- wp_operand (Eunop o e ty) Q.
+
+    Let with_tu (P : translation_unit -> mpred) : mpred :=
+          Exists tu, [| tu ⊧ resolve |] ** P tu.
 
     (** `++e`
         https://eel.is/c++draft/expr.pre.incr#1
@@ -285,7 +288,7 @@ Module Type Expr.
          match companion_type eety with
          | Some cty =>
           wp_lval e (fun a free => Exists v' v'',
-              (eval_binop Badd eety cty (erase_qualifiers ty) v' (Vint 1) v'' ** True) //\\
+              (with_tu $ fun tu => eval_binop tu Badd eety cty (erase_qualifiers ty) v' (Vint 1) v'' ** True) //\\
               (a |-> primR eety 1 v' **
                 (a |-> primR eety 1 v'' -* Q a free)))
          | None => False
@@ -301,7 +304,7 @@ Module Type Expr.
          match companion_type eety with
          | Some cty =>
           wp_lval e (fun a free => Exists v' v'',
-              (eval_binop Bsub eety cty (erase_qualifiers ty) v' (Vint 1) v'' ** True) //\\
+              (with_tu $ fun tu => eval_binop tu Bsub eety cty (erase_qualifiers ty) v' (Vint 1) v'' ** True) //\\
               (a |-> primR eety 1 v' **
                 (a |-> primR eety 1 v'' -* Q a free)))
          | None => False
@@ -317,7 +320,7 @@ Module Type Expr.
          match companion_type eety with
          | Some cty =>
              wp_lval e (fun a free => Exists v', Exists v'',
-                          (eval_binop Badd eety cty
+                          (with_tu $ fun tu => eval_binop tu Badd eety cty
                              (erase_qualifiers ty) v' (Vint 1) v'' ** True) //\\
                             (a |-> primR eety 1 v' **
                                (a |-> primR eety 1 v'' -* Q v' free)))
@@ -334,7 +337,7 @@ Module Type Expr.
          match companion_type eety with
          | Some cty =>
              wp_lval e (fun a free => Exists v', Exists v'',
-                          (eval_binop Bsub eety cty
+                          (with_tu $ fun tu => eval_binop tu Bsub eety cty
                              (erase_qualifiers ty) v' (Vint 1) v'' ** True) //\\
                             (a |-> primR eety 1 v' **
                                (a |-> primR eety 1 v'' -* Q v' free)))
@@ -347,7 +350,7 @@ Module Type Expr.
     Axiom wp_operand_binop : forall o e1 e2 ty Q,
         nd_seq (wp_operand e1) (wp_operand e2) (fun '(v1,v2) free =>
           Exists v',
-            (eval_binop o
+            (with_tu $ fun tu => eval_binop tu o
                 (drop_qualifiers (type_of e1)) (drop_qualifiers (type_of e2))
                 (drop_qualifiers ty) v1 v2 v' ** True) //\\
             Q v' free)
@@ -369,7 +372,7 @@ Module Type Expr.
     Axiom wp_lval_bop_assign : forall ty o l r Q,
         nd_seq (wp_lval l) (wp_operand r) (fun '(la, rv) free =>
              (Exists v v', la |-> primR (erase_qualifiers ty) 1 v **
-                 ((eval_binop o (erase_qualifiers (type_of l)) (erase_qualifiers (type_of r)) (erase_qualifiers (type_of l)) v rv v' ** True) //\\
+                 (with_tu $ fun tu => (eval_binop tu o (erase_qualifiers (type_of l)) (erase_qualifiers (type_of r)) (erase_qualifiers (type_of l)) v rv v' ** True) //\\
                  (la |-> primR (erase_qualifiers ty) 1 v' -* Q la free))))
         |-- wp_lval (Eassign_op o l r ty) Q.
 
@@ -509,10 +512,11 @@ Module Type Expr.
         - [int] -> [short]
         - [short] -> [long]
         - [int] -> [unsigned int]
+        - [enum Xxx] -> [int]
      *)
     Axiom wp_operand_cast_integral : forall e t Q,
         wp_operand e (fun v free =>
-           Exists v', [| conv_int (type_of e) t v v' |] ** Q v' free)
+           Exists v', [| exists tu, tu ⊧ resolve /\ conv_int tu (type_of e) t v v' |] ** Q v' free)
         |-- wp_operand (Ecast Cintegral Prvalue e t) Q.
 
     Axiom wp_operand_cast_null : forall e t Q,
